module Data.Binary.Subtraction where

open import Data.Binary.Definition
open import Data.Binary.Decrement
open import Data.Binary.Double
open import Data.Binary.Helpers

ones : โ โ ๐น โ ๐น
ones zero    xs = xs
ones (suc n) xs = ones n (1แต xs)

infixl 7 _+1ร2^suc_ _ร2^suc_
_+1ร2^suc_ : ๐น โ โ โ ๐น
xs +1ร2^suc n = 2แต ones n xs

_ร2^suc_ : ๐น โ โ โ ๐น
0แต      ร2^suc n = 0แต
(1แต xs) ร2^suc n = 2ร xs +1ร2^suc n
(2แต xs) ร2^suc n = xs +1ร2^suc suc n

data ๐นยฑ : Set where
  neg : ๐นยฑ
  +[_] : ๐น โ ๐นยฑ

+[_]+1ร2^suc_ : ๐นยฑ โ โ โ ๐นยฑ
+[ neg    ]+1ร2^suc n = neg
+[ +[ x ] ]+1ร2^suc n = +[ 2แต ones n x ]

1แต+[_] : ๐นยฑ โ ๐นยฑ
1แต+[ neg ] = neg
1แต+[ +[ x ] ] = +[ 1แต x ]

abs : ๐นยฑ โ ๐น
abs neg = 0แต
abs +[ x ] = x

mutual
  -- subแตโ n x y = (x - (y + 1)) ร 2โฟโบยน
  subแตโ : โ โ ๐น โ ๐น โ ๐นยฑ
  subแตโ n 0แต      _       = neg
  subแตโ n (1แต xs) 0แต      = +[ xs ร2^suc suc n ]
  subแตโ n (2แต xs) 0แต      = +[ 2ร xs +1ร2^suc n ]
  subแตโ n (1แต xs) (1แต ys) = +[ subแตโ 0 xs ys ]+1ร2^suc n
  subแตโ n (2แต xs) (2แต ys) = +[ subแตโ 0 xs ys ]+1ร2^suc n
  subแตโ n (1แต xs) (2แต ys) = subแตโ (suc n) xs ys
  subแตโ n (2แต xs) (1แต ys) = subแต  (suc n) xs ys

  -- subแต n x y = (x - y) ร 2โฟโบยน
  subแต : โ โ ๐น โ ๐น โ ๐นยฑ
  subแต n xs      0แต      = +[ xs ร2^suc n ]
  subแต _ 0แต      (1แต _)  = neg
  subแต _ 0แต      (2แต _)  = neg
  subแต n (1แต xs) (1แต ys) = subแต (suc n) xs ys
  subแต n (2แต xs) (2แต ys) = subแต (suc n) xs ys
  subแต n (1แต xs) (2แต ys) = +[ subแตโ 0 xs ys ]+1ร2^suc n
  subแต n (2แต xs) (1แต ys) = +[ subแต  0 xs ys ]+1ร2^suc n

mutual
  -- subโ x y = x - (y + 1)
  subโ : ๐น โ ๐น โ ๐นยฑ
  subโ 0แต      _       = neg
  subโ (1แต xs) 0แต      = +[ 2ร xs ]
  subโ (2แต xs) 0แต      = +[ 1แต xs ]
  subโ (1แต xs) (1แต ys) = 1แต+[ subโ xs ys ]
  subโ (2แต xs) (2แต ys) = 1แต+[ subโ xs ys ]
  subโ (1แต xs) (2แต ys) = subแตโ 0 xs ys
  subโ (2แต xs) (1แต ys) = subแต  0 xs ys

  -- sub x y = x - y
  sub : ๐น โ ๐น โ ๐นยฑ
  sub xs      0แต      = +[ xs ]
  sub 0แต      (1แต _)  = neg
  sub 0แต      (2แต _)  = neg
  sub (1แต xs) (1แต ys) = subแต 0 xs ys
  sub (2แต xs) (2แต ys) = subแต 0 xs ys
  sub (1แต xs) (2แต ys) = 1แต+[ subโ xs ys ]
  sub (2แต xs) (1แต ys) = 1แต+[ sub  xs ys ]

infixl 6 _-_
_-_ : ๐น โ ๐น โ ๐น
n - m = abs (sub n m)
