{-# OPTIONS --cubical #-}

module Data.Binary.Properties.Subtraction where

open import Data.Binary.Definition
open import Data.Binary.Addition
open import Data.Binary.Properties.Addition using (+-cong)
open import Data.Binary.Multiplication
open import Data.Binary.Conversion
import Agda.Builtin.Nat as โ

open import Data.Binary.Properties.Isomorphism

open import Data.Binary.Helpers
open import Data.Binary.Properties.Helpers
open import Data.Binary.Properties.Double
open import Data.Binary.Double
open import Data.Binary.Subtraction

_-โฒ_ : โ โ โ โ Maybe โ
n     -โฒ zero  = just n
zero  -โฒ suc _ = nothing
suc n -โฒ suc m = n -โฒ m

1แตโ : โ โ โ
1แตโ n = suc (n โ.* 2)

-โฒโฟcong : โ n m โ from-maybe 0 (n -โฒ m) โก n โ.- m
-โฒโฟcong n zero    = refl
-โฒโฟcong zero (suc m) = refl
-โฒโฟcong (suc n) (suc m) = -โฒโฟcong n m

โฆ_โโงโฒ : Maybe ๐น โ Maybe โ
โฆ_โโงโฒ = map-maybe โฆ_โโง

exp2 : โ โ โ โ โ
exp2 zero    x = x
exp2 (suc n) x = exp2 n x โ.* 2

exp2-๐น : โ โ ๐น โ ๐น
exp2-๐น zero    xs = xs
exp2-๐น (suc n) xs = exp2-๐น n (2ร xs)

exp2-๐น-0แต : โ n โ exp2-๐น n 0แต โก 0แต
exp2-๐น-0แต zero = refl
exp2-๐น-0แต (suc n) = exp2-๐น-0แต n

exp2-๐น-2แต : โ n xs โ exp2-๐น n (2แต xs) โก xs +1ร2^suc n
exp2-๐น-2แต zero 0แต = refl
exp2-๐น-2แต zero (1แต xs) = refl
exp2-๐น-2แต zero (2แต xs) = refl
exp2-๐น-2แต (suc n) xs = exp2-๐น-2แต n (1แต xs)

exp2-๐น-ร2^suc : โ n xs โ exp2-๐น (suc n) xs โก xs ร2^suc n
exp2-๐น-ร2^suc n 0แต      = exp2-๐น-0แต n
exp2-๐น-ร2^suc n (1แต xs) = exp2-๐น-2แต n (2ร xs)
exp2-๐น-ร2^suc n (2แต xs) = exp2-๐น-2แต n (1แต xs)

exp2-assoc : โ n m โ exp2 n (m โ.* 2) โก exp2 n m โ.* 2
exp2-assoc zero m = refl
exp2-assoc (suc n) m = cong (โ._* 2) (exp2-assoc n m)

exp2-๐น-cong : โ n xs โ โฆ exp2-๐น n xs โโง โก exp2 n โฆ xs โโง
exp2-๐น-cong zero xs = refl
exp2-๐น-cong (suc n) xs = exp2-๐น-cong n (2ร xs) โ cong (exp2 n) (double-cong xs) โ exp2-assoc n โฆ xs โโง

ร2^suc-cong : โ n xs โ โฆ xs ร2^suc n โโง โก exp2 (suc n) โฆ xs โโง
ร2^suc-cong n xs = cong โฆ_โโง (sym (exp2-๐น-ร2^suc n xs)) โ exp2-๐น-cong (suc n) xs

maybe-fuse : {A B C : Set} (c : B โ C) (f : A โ B) (b : B) (x : Maybe A)
           โ c (maybe f b x) โก maybe (c โ f) (c b) x
maybe-fuse _ _ _ nothing  = refl
maybe-fuse _ _ _ (just _) = refl

map-maybe-comp : {A B C : Set} (f : A โ B) (b : B) (g : C โ A) (x : Maybe C) โ maybe f b (map-maybe g x) โก maybe (f โ g) b x
map-maybe-comp f b g = maybe-fuse (maybe f b) _ _

1แตz-lemma : โ n โ โฆ map-maybe 1แต_ n โโงโฒ โก map-maybe 1แตโ (map-maybe โฆ_โโง n)
1แตz-lemma nothing  = refl
1แตz-lemma (just x) = refl

1แตzs-distribโฟ-โฒ : โ x y โ map-maybe 1แตโ (x -โฒ suc y) โก  (x โ.* 2) -โฒ suc (y โ.* 2)
1แตzs-distribโฟ-โฒ zero y = refl
1แตzs-distribโฟ-โฒ (suc x) zero = refl
1แตzs-distribโฟ-โฒ (suc x) (suc y) = 1แตzs-distribโฟ-โฒ x y

2แตzs-distribโฟ-โฒ : โ x y โ map-maybe (โ._* 2) (x -โฒ suc y) โก  (x โ.* 2) -โฒ suc (suc (y โ.* 2))
2แตzs-distribโฟ-โฒ zero y = refl
2แตzs-distribโฟ-โฒ (suc x) zero = refl
2แตzs-distribโฟ-โฒ (suc x) (suc y) = 2แตzs-distribโฟ-โฒ x y

1แตsz-distribโฟ-โฒ : โ x y โ map-maybe 1แตโ (x -โฒ y) โก suc (x โ.* 2) -โฒ (y โ.* 2)
1แตsz-distribโฟ-โฒ zero zero = refl
1แตsz-distribโฟ-โฒ zero (suc y) = refl
1แตsz-distribโฟ-โฒ (suc x) zero = refl
1แตsz-distribโฟ-โฒ (suc x) (suc y) = 1แตsz-distribโฟ-โฒ x y

+-congโฟ-โฒ : โ n x y โ (n โ.+ x) -โฒ (n โ.+ y) โก x -โฒ y
+-congโฟ-โฒ zero x y = refl
+-congโฟ-โฒ (suc n) x y = +-congโฟ-โฒ n x y

*-distribโฟ-โฒ : โ n x y โ map-maybe (โ._* suc n) (x -โฒ y) โก (x โ.* suc n) -โฒ (y โ.* suc n)
*-distribโฟ-โฒ n zero zero = refl
*-distribโฟ-โฒ n zero (suc y) = refl
*-distribโฟ-โฒ n (suc x) zero = refl
*-distribโฟ-โฒ n (suc x) (suc y) = *-distribโฟ-โฒ n x y โ sym (+-congโฟ-โฒ n _ _)

-โฒโฟ*2-suc : โ x y โ map-maybe suc ((x โ.* 2) -โฒ (y โ.* 2)) โก suc (x โ.* 2) -โฒ (y โ.* 2)
-โฒโฟ*2-suc zero zero = refl
-โฒโฟ*2-suc zero (suc y) = refl
-โฒโฟ*2-suc (suc x) zero = refl
-โฒโฟ*2-suc (suc x) (suc y) = -โฒโฟ*2-suc x y

-โฒโฟsuc-*2 : โ x y โ map-maybe (suc โ (โ._* 2)) (x -โฒ suc y) โก (x โ.* 2) -โฒ suc (y โ.* 2)
-โฒโฟsuc-*2 zero zero = refl
-โฒโฟsuc-*2 zero (suc y) = refl
-โฒโฟsuc-*2 (suc x) zero = refl
-โฒโฟsuc-*2 (suc x) (suc y) = -โฒโฟsuc-*2 x y

+1ร2^suc-cong : โ n xs โ โฆ xs +1ร2^suc n โโง โก exp2 (suc n) (suc โฆ xs โโง)
+1ร2^suc-cong n xs = cong โฆ_โโง (sym (exp2-๐น-2แต n xs)) โ exp2-๐น-cong n (2แต xs) โ exp2-assoc n (suc โฆ xs โโง)

exp-suc-lemma : โ n xs ys โ map-maybe (ฮป x โ exp2 n x โ.* 2 โ.* 2) (xs -โฒ ys) โก
                  map-maybe (ฮป x โ exp2 n x โ.* 2)
                  ((xs โ.* 2) -โฒ (ys โ.* 2))
exp-suc-lemma n xs ys = cong (flip map-maybe (xs -โฒ ys)) (funExt (ฮป x โ cong (โ._* 2) (sym (exp2-assoc n x)))) โ sym (map-maybe-comp _ _ _ (xs -โฒ ys)) โ cong (map-maybe (exp2 (suc n))) (*-distribโฟ-โฒ 1 xs ys)

subแตโ-0-cong : โ n xs ys โ โฆ map-maybe (_+1ร2^suc n) (subแตโ 0 xs ys) โโงโฒ โก map-maybe (exp2 (suc n)) ((โฆ xs โโง โ.* 2) -โฒ suc (โฆ ys โโง โ.* 2))
subแต-0-cong : โ n xs ys โ โฆ map-maybe (_+1ร2^suc n) (subแต 0 xs ys) โโงโฒ โก map-maybe (exp2 (suc n)) (suc (โฆ xs โโง โ.* 2) -โฒ (โฆ ys โโง โ.* 2))
subแต-cong  : โ n xs ys โ โฆ subแต  n xs ys โโงโฒ โก map-maybe (exp2 (suc n)) (โฆ xs โโง -โฒ โฆ ys โโง)
subแตโ-cong : โ n xs ys โ โฆ subแตโ n xs ys โโงโฒ โก map-maybe (exp2 (suc n)) (โฆ xs โโง -โฒ suc โฆ ys โโง)
subโ-cong  : โ   xs ys โ โฆ subโ xs ys โโงโฒ โก โฆ xs โโง -โฒ suc โฆ ys โโง
sub-cong   : โ   xs ys โ โฆ sub xs ys โโงโฒ โก โฆ xs โโง -โฒ โฆ ys โโง

subแตโ-0-cong n xs ys =
  โฆ map-maybe (_+1ร2^suc n) (subแตโ 0 xs ys) โโงโฒ โกโจ map-maybe-comp _ _ _ (subแตโ 0 xs ys) โฉ
  map-maybe (โฆ_โโง โ (_+1ร2^suc n)) (subแตโ 0 xs ys) โกโจ cong (flip map-maybe (subแตโ 0 xs ys)) (funExt (+1ร2^suc-cong n)) โฉ
  map-maybe (exp2 (suc n) โ suc โ โฆ_โโง) (subแตโ 0 xs ys) โกหโจ map-maybe-comp _ _ _ (subแตโ 0 xs ys) โฉ
  map-maybe (exp2 (suc n) โ suc) โฆ subแตโ 0 xs ys โโงโฒ โกโจ cong (map-maybe (exp2 (suc n) โ suc)) (subแตโ-cong 0 xs ys) โฉ
  map-maybe (exp2 (suc n) โ suc) (map-maybe (exp2 1) (โฆ xs โโง -โฒ suc โฆ ys โโง)) โกโจ map-maybe-comp _ _ _ (โฆ xs โโง -โฒ suc โฆ ys โโง) โฉ
  map-maybe (exp2 (suc n) โ suc โ exp2 1) (โฆ xs โโง -โฒ suc โฆ ys โโง) โกหโจ map-maybe-comp _ _ _ (โฆ xs โโง -โฒ suc โฆ ys โโง) โฉ
  map-maybe (exp2 (suc n)) (map-maybe (suc โ exp2 1) (โฆ xs โโง -โฒ suc โฆ ys โโง)) โกโจ cong (map-maybe (exp2 (suc n))) (-โฒโฟsuc-*2 โฆ xs โโง โฆ ys โโง) โฉ
  map-maybe (exp2 (suc n)) ((โฆ xs โโง โ.* 2) -โฒ suc (โฆ ys โโง โ.* 2)) โ

subแต-0-cong n xs ys =
  โฆ map-maybe (_+1ร2^suc n) (subแต 0 xs ys) โโงโฒ โกโจ map-maybe-comp _ _ _ (subแต 0 xs ys) โฉ
  map-maybe (โฆ_โโง โ (_+1ร2^suc n)) (subแต 0 xs ys) โกโจ cong (flip map-maybe (subแต 0 xs ys)) (funExt (+1ร2^suc-cong n)) โฉ
  map-maybe (exp2 (suc n) โ suc โ โฆ_โโง) (subแต 0 xs ys) โกหโจ map-maybe-comp _ _ _ (subแต 0 xs ys) โฉ
  map-maybe (exp2 (suc n) โ suc) โฆ subแต 0 xs ys โโงโฒ โกโจ cong (map-maybe (exp2 (suc n) โ suc)) (subแต-cong 0 xs ys) โฉ
  map-maybe (exp2 (suc n) โ suc) (map-maybe (exp2 1) (โฆ xs โโง -โฒ โฆ ys โโง)) โกโจ map-maybe-comp _ _ _ (โฆ xs โโง -โฒ โฆ ys โโง) โฉ
  map-maybe (exp2 (suc n) โ suc โ exp2 1) (โฆ xs โโง -โฒ โฆ ys โโง) โกหโจ map-maybe-comp _ _ _ (โฆ xs โโง -โฒ โฆ ys โโง) โฉ
  map-maybe (exp2 (suc n)) (map-maybe (suc โ exp2 1) (โฆ xs โโง -โฒ โฆ ys โโง)) โกหโจ cong (map-maybe (exp2 (suc n))) (map-maybe-comp _ _ _ (โฆ xs โโง -โฒ โฆ ys โโง)) โฉ
  map-maybe (exp2 (suc n)) (map-maybe suc (map-maybe (exp2 1) (โฆ xs โโง -โฒ โฆ ys โโง))) โกโจ cong (map-maybe (exp2 (suc n)) โ map-maybe suc) (*-distribโฟ-โฒ 1 โฆ xs โโง โฆ ys โโง) โฉ
  map-maybe (exp2 (suc n)) (map-maybe suc (exp2 1 โฆ xs โโง -โฒ exp2 1 โฆ ys โโง)) โกโจ cong (map-maybe (exp2 (suc n))) (-โฒโฟ*2-suc โฆ xs โโง โฆ ys โโง) โฉ
  map-maybe (exp2 (suc n)) (suc (โฆ xs โโง โ.* 2) -โฒ (โฆ ys โโง โ.* 2)) โ

subแต-cong n xs      0แต      = cong just (ร2^suc-cong n xs)
subแต-cong n 0แต      (1แต ys) = refl
subแต-cong n 0แต      (2แต ys) = refl
subแต-cong n (1แต xs) (1แต ys) = subแต-cong (suc n) xs ys โ exp-suc-lemma n โฆ xs โโง โฆ ys โโง
subแต-cong n (1แต xs) (2แต ys) = subแตโ-0-cong n xs ys
subแต-cong n (2แต xs) (1แต ys) = subแต-0-cong n xs ys

subแต-cong n (2แต xs) (2แต ys) = subแต-cong (suc n) xs ys โ exp-suc-lemma n โฆ xs โโง โฆ ys โโง

subแตโ-cong n 0แต      _       = refl
subแตโ-cong n (1แต xs) 0แต      = cong just (ร2^suc-cong (suc n) xs โ cong (โ._* 2) (sym (exp2-assoc n โฆ xs โโง)))
subแตโ-cong n (1แต xs) (1แต ys) = subแตโ-0-cong n xs ys
subแตโ-cong n (1แต xs) (2แต ys) = subแตโ-cong (suc n) xs ys โ exp-suc-lemma n โฆ xs โโง (suc โฆ ys โโง)
subแตโ-cong n (2แต xs) 0แต      = cong just (+1ร2^suc-cong n (2ร xs) โ cong (ฮป e โ exp2 n (suc e) โ.* 2) (double-cong xs))
subแตโ-cong n (2แต xs) (1แต ys) = subแต-cong (suc n) xs ys โ exp-suc-lemma n โฆ xs โโง โฆ ys โโง
subแตโ-cong n (2แต xs) (2แต ys) = subแตโ-0-cong n xs ys

subโ-cong 0แต      _       = refl
subโ-cong (1แต xs) 0แต      = cong just (double-cong xs)
subโ-cong (1แต xs) (1แต ys) = 1แตz-lemma (subโ xs ys) โ cong (map-maybe 1แตโ) (subโ-cong xs ys) โ 1แตzs-distribโฟ-โฒ โฆ xs โโง โฆ ys โโง
subโ-cong (1แต xs) (2แต ys) = subแตโ-cong 0 xs ys โ 2แตzs-distribโฟ-โฒ โฆ xs โโง โฆ ys โโง
subโ-cong (2แต xs) 0แต      = refl
subโ-cong (2แต xs) (1แต ys) = subแต-cong 0 xs ys โ *-distribโฟ-โฒ 1 โฆ xs โโง โฆ ys โโง
subโ-cong (2แต xs) (2แต ys) = 1แตz-lemma (subโ xs ys) โ cong (map-maybe 1แตโ) (subโ-cong xs ys) โ 1แตzs-distribโฟ-โฒ โฆ xs โโง โฆ ys โโง

sub-cong xs 0แต           = refl
sub-cong 0แต      (1แต _)  = refl
sub-cong 0แต      (2แต _)  = refl
sub-cong (1แต xs) (1แต ys) = subแต-cong 0 xs ys โ *-distribโฟ-โฒ 1 โฆ xs โโง โฆ ys โโง
sub-cong (2แต xs) (2แต ys) = subแต-cong 0 xs ys โ *-distribโฟ-โฒ 1 โฆ xs โโง โฆ ys โโง
sub-cong (1แต xs) (2แต ys) = 1แตz-lemma (subโ xs ys) โ cong (map-maybe 1แตโ) (subโ-cong xs ys) โ 1แตzs-distribโฟ-โฒ โฆ xs โโง โฆ ys โโง
sub-cong (2แต xs) (1แต ys) = 1แตz-lemma (sub xs ys) โ cong (map-maybe 1แตโ) (sub-cong xs ys) โ 1แตsz-distribโฟ-โฒ โฆ xs โโง โฆ ys โโง

-โฟcong : โ xs ys โ โฆ xs - ys โโง โก โฆ xs โโง โ.- โฆ ys โโง
-โฟcong x y = maybe-fuse โฆ_โโง _ _ (sub x y)
           โ sym (map-maybe-comp _ _ โฆ_โโง (sub x y))
           โ cong (from-maybe 0) (sub-cong x y)
           โ -โฒโฟcong โฆ x โโง โฆ y โโง
